GVN.v
@@ -1,0 +1,442 @@
+Require Import Bool.
+Require Import Sorting.Permutation.
+Require Import Omega.
+Require Import sflib.
+
+Require Import Common.
+Require Import Value.
+Require Import Lang.
+Require Import Memory.
+Require Import State.
+Require Import LoadStore.
+Require Import SmallStep.
+Require Import Refinement.
+Require Import TwinExecution.
+
+Module Ir.
+
+Module GVN.
+
+Inductive physicalized_ptr: Ir.Memory.t -> Ir.val -> Ir.val -> Prop :=
+| ps_base:
+    forall m p1 p2
+           (HP2:Some p2 = Ir.ptr_to_phy m p1),
+      physicalized_ptr m (Ir.ptr p1) (Ir.ptr p2)
+| ps_gep:
+    forall m p1 p2 idx t inb p1' p2'
+           (HBASE:physicalized_ptr m (Ir.ptr p1) (Ir.ptr p2))
+           (HP1':p1' = Ir.SmallStep.gep p1 idx t m inb)
+           (HP2':p2' = Ir.SmallStep.gep p2 idx t m inb),
+      physicalized_ptr m p1' p2'.
+
+
+Lemma eq_update_reg_and_incrpc2:
+  forall md1 md2 st r v i1 i2
+      (HINST1: Some i1 = Ir.Config.cur_inst md1 st)
+      (HINST2: Some i2 = Ir.Config.cur_inst md2 st),
+    Ir.Config.eq
+      (Ir.SmallStep.update_reg_and_incrpc md1 st r v)
+      (Ir.SmallStep.update_reg_and_incrpc md2 st r v).
+Proof.
+  intros.
+  unfold Ir.Config.cur_inst in HINST1.
+  unfold Ir.Config.cur_inst in HINST2.
+  split.
+  { unfold Ir.SmallStep.update_reg_and_incrpc.
+    unfold Ir.SmallStep.incrpc.
+    des_ifs;
+      repeat (rewrite Ir.Config.m_update_pc);
+      unfold Ir.Config.update_rval; des_ifs.
+  }
+  split.
+  { unfold Ir.Config.cur_fdef_pc in HINST1.
+    unfold Ir.Config.cur_fdef_pc in HINST2.
+    des_ifs.
+    unfold Ir.IRFunction.get_inst in HINST1.
+    unfold Ir.IRFunction.get_inst in HINST2.
+    destruct p1; try congruence.
+    des_ifs.
+    unfold Ir.SmallStep.update_reg_and_incrpc.
+    unfold Ir.SmallStep.incrpc.
+    rewrite Ir.Config.cur_fdef_pc_update_rval.
+    rewrite Ir.Config.cur_fdef_pc_update_rval.
+    unfold Ir.Config.cur_fdef_pc.
+    rewrite Heq0.
+    rewrite Heq1.
+    rewrite Heq2.
+    rewrite Heq3.
+    unfold Ir.IRFunction.next_trivial_pc.
+    rewrite Heq5.
+    rewrite Heq.
+    rewrite Heq6.
+    rewrite Heq4.
+    apply Ir.Stack.eq_refl.
+  }
+  split.
+  { unfold Ir.SmallStep.update_reg_and_incrpc.
+    unfold Ir.SmallStep.incrpc.
+    des_ifs;
+      unfold Ir.Config.update_pc; unfold Ir.Config.update_rval;
+      des_ifs.
+  }
+  { unfold Ir.SmallStep.update_reg_and_incrpc.
+    unfold Ir.SmallStep.incrpc.
+    des_ifs;
+      unfold Ir.Config.update_pc; unfold Ir.Config.update_rval;
+      des_ifs.
+  }
+Qed.
+
+Lemma physicalized_ptr_nonlog:
+  forall m p1 p2
+         (HPP:physicalized_ptr m (Ir.ptr p1) (Ir.ptr p2)),
+    ~ exists l o, p2 = Ir.plog l o.
+Proof.
+  intros.
+  remember (Ir.ptr p1) as v1.
+  remember (Ir.ptr p2) as v2.
+  generalize dependent p1.
+  generalize dependent p2.
+  induction HPP.
+  { intros. inv Heqv1. inv Heqv2.
+    unfold Ir.ptr_to_phy in HP2.
+    destruct p3.
+    { unfold Ir.log_to_phy in HP2.
+      destruct (Ir.Memory.get m b).
+      { intros HH. destruct HH. destruct H. rewrite H in HP2.
+        congruence. }
+      { congruence. }
+    }
+    { intros HH. destruct HH. destruct H. rewrite H in HP2.
+      congruence. }
+  }
+  { intros. inv Heqv1. inv Heqv2.
+    intros HH.
+    destruct HH. destruct H0. rewrite H0 in H1.
+    eapply IHHPP.
+    reflexivity. reflexivity.
+    unfold Ir.SmallStep.gep in H1.
+    destruct p2.
+    { destruct inb.
+      { des_ifs.
+        eexists. eexists . reflexivity. }
+      { eexists. eexists . reflexivity. }
+    }
+    { destruct inb.
+      { des_ifs. }
+      { congruence. }
+    }
+  }
+Qed.
+
+Lemma physicalized_ptr_phy:
+  forall m o1 Is1 cid1 o2 Is2 cid2 v1 v2
+         (HPP:physicalized_ptr m v1 v2)
+         (HV1:v1 = Ir.ptr (Ir.pphy o1 Is1 cid1))
+         (HV2:v2 = Ir.ptr (Ir.pphy o2 Is2 cid2)),
+    o1 = o2 /\ lsubseq Is1 Is2 /\ cid2 = None.
+Proof.
+  intros.
+  generalize dependent o1.
+  generalize dependent Is1.
+  generalize dependent cid1.
+  generalize dependent o2.
+  generalize dependent Is2.
+  generalize dependent cid2.
+  induction HPP.
+  { intros.
+    inv HV1.
+    unfold Ir.ptr_to_phy in HP2. inv HP2.
+    inv HV2.
+    split. reflexivity.
+    split. constructor.
+    reflexivity.
+  }
+  { intros.
+    destruct p2'; try congruence.
+    destruct p1'; try congruence.
+    inv HV2.
+    inv HV1.
+    destruct p2.
+    { eapply physicalized_ptr_nonlog in HPP.
+      exfalso. apply HPP. eexists. eexists. reflexivity.
+    }
+    { unfold Ir.SmallStep.gep in HP1'.
+      des_ifs.
+      {
+        exploit IHHPP.
+        { reflexivity. }
+        { reflexivity. }
+        intros HH.
+        unfold Ir.SmallStep.gep in HP2'.
+        des_ifs.
+        { inv HH. destruct H0.
+          split. reflexivity.
+          split. constructor. constructor. assumption.
+          assumption.
+        }
+      }
+      { exploit IHHPP; try reflexivity.
+        intros HH.
+        inv HH. destruct H0.
+        unfold Ir.SmallStep.gep in HP2'.
+        des_ifs.
+        split. reflexivity.
+        split. constructor. constructor. assumption.
+        reflexivity.
+      }
+      { exploit IHHPP; try reflexivity.
+        intros HH.
+        inv HH. destruct H0.
+        unfold Ir.SmallStep.gep in HP2'.
+        des_ifs.
+      }
+    }
+  }
+Qed.
+
+Lemma physicalized_ptr_log:
+  forall m l1 o1 o2 Is2 cid2 v1 v2 mb
+         (HPP:physicalized_ptr m v1 v2)
+         (HV1:v1 = Ir.ptr (Ir.plog l1 o1))
+         (HV2:v2 = Ir.ptr (Ir.pphy o2 Is2 cid2))
+         (HGET:Some mb = Ir.Memory.get m l1),
+    (Ir.MemBlock.addr mb + o1) mod Ir.MEMSZ = o2.
+Proof.
+  intros.
+  generalize dependent l1.
+  generalize dependent o1.
+  generalize dependent o2.
+  generalize dependent Is2.
+  generalize dependent cid2.
+  induction HPP.
+  { intros.
+    inv HV1.
+    unfold Ir.ptr_to_phy in HP2. inv HP2.
+    inv HV2.
+    unfold Ir.log_to_phy in H0.
+    rewrite <- HGET in H0.
+    congruence.
+  }
+  { intros.
+    destruct p2'; try congruence.
+    destruct p1'; try congruence.
+    inv HV2.
+    inv HV1.
+    destruct p2.
+    { eapply physicalized_ptr_nonlog in HPP.
+      exfalso. apply HPP. eexists. eexists. reflexivity.
+    }
+    { unfold Ir.SmallStep.gep in HP1'.
+      des_ifs.
+      {
+        exploit IHHPP.
+        { reflexivity. }
+        { reflexivity. }
+        { assumption. }
+        intros HH.
+        unfold Ir.SmallStep.gep in HP2'.
+        destruct ((idx * N.of_nat (Ir.ty_bytesz t) <?
+            N.shiftl 1 (N.of_nat Ir.PTRSZ - 1))%N) eqn:H11.
+        { (* positive offset add *)
+          destruct (N.to_nat
+             (Ir.SmallStep.twos_compl_add (N.of_nat n)
+                (idx * N.of_nat (Ir.ty_bytesz t)) Ir.PTRSZ) <? Ir.MEMSZ) eqn:H2.
+          { assert 
+        des_ifs.
+        { inv HH. destruct H0.
+          split. reflexivity.
+          split. constructor. constructor. assumption.
+          assumption.
+        }
+      }
+      { exploit IHHPP; try reflexivity.
+        intros HH.
+        inv HH. destruct H0.
+        unfold Ir.SmallStep.gep in HP2'.
+        des_ifs.
+        split. reflexivity.
+        split. constructor. constructor. assumption.
+        reflexivity.
+      }
+      { exploit IHHPP; try reflexivity.
+        intros HH.
+        inv HH. destruct H0.
+        unfold Ir.SmallStep.gep in HP2'.
+        des_ifs.
+      }
+    }
+  }
+Qed.
+
+Lemma get_deref_physicalized_ptr:
+  forall md st sz p1 p2
+         (HWF:Ir.Config.wf md st)
+         (HSZ:sz> 0)
+         (HPP:physicalized_ptr (Ir.Config.m st) (Ir.ptr p1) (Ir.ptr p2)),
+    forall blk, Ir.get_deref (Ir.Config.m st) p1 sz = [blk] ->
+                Ir.get_deref (Ir.Config.m st) p2 sz = [blk].
+Proof.
+  intros.
+  inv HWF.
+  remember (Ir.ptr p1) as v1.
+  remember (Ir.ptr p2) as v2.
+  generalize dependent blk.
+  generalize dependent p1.
+  generalize dependent p2.
+  clear wf_cid_to_f.
+  clear wf_cid_to_f2.
+  clear wf_stack.
+  clear wf_no_bogus_ptr.
+  clear wf_no_bogus_ptr_mem.
+  induction HPP.
+  { intros.
+    rename p0 into p2'.
+    rename p3 into p1'.
+    inv Heqv2. inv Heqv1.
+    eapply Ir.get_deref_ptr_phy_same.
+    { eassumption. }
+    { omega. }
+    { eassumption. }
+    { congruence. }
+  }
+  { intros.
+    subst p2'.
+    subst p1'.
+    assert (HA := IHHPP wf_m p2 (eq_refl (Ir.ptr p2)) p1 ).
+    rename p0 into p2'.
+    rename p3 into p1'.
+    clear IHHPP.
+    unfold Ir.SmallStep.gep in Heqv1.
+    destruct p1.
+    { (* p1 was log. *)
+      destruct inb eqn:HINB.
+      { (* inbounds *)
+        des_ifs.
+        (* okay, how about p2? *)
+        unfold Ir.SmallStep.gep in Heqv2.
+        destruct p2.
+        { admit. }
+        { (* p2 is phy. *)
+          des_ifs.
+          { (* added offset was positive. *)
+            eapply Ir.get_deref_ptr_phy_same in H; try assumption.
+            2: unfold Ir.ptr_to_phy.
+            2: unfold Ir.log_to_phy.
+            2: rewrite Heq.
+            2: reflexivity.
+            (* okay, Ir.plog b n and Ir.pphy (n0 l o) has same integer repr. *)
+            
+            assert (Ir.get_deref m (Ir.plog b n) sz = [(b, t0, n)]).
+            { unfold Ir.get_deref.
+              rewrite Heq.
+              unfold Ir.get_deref in H.
+              rewrite Heq in H.
+              destruct (Ir.MemBlock.alive t0).
+              { simpl. 
+          { (* added offset was negative - no check *)
+    
+    
+    
+
+Theorem load_refines:
+  forall md1 md2 (* md2 is an optimized program *)
+         st r retty opptr1 opptr2 v1 v2 sr1 sr2
+         (HWF1:Ir.Config.wf md1 st)
+         (HWF2:Ir.Config.wf md2 st) (* State st is wellformed on two modules *)
+         (* Two loads on a same state(including same PC) *)
+         (HINST1:Some (Ir.Inst.iload r retty opptr1) = Ir.Config.cur_inst md1 st)
+         (HINST2:Some (Ir.Inst.iload r retty opptr2) = Ir.Config.cur_inst md2 st)
+         (* Has a good relation between pointer operands *)
+         (HOP1:Ir.Config.get_val st opptr1 = Some v1)
+         (HOP2:Ir.Config.get_val st opptr2 = Some v2)
+         (HPP:physicalized_ptr (Ir.Config.m st) v1 v2)
+         (* And.. have a step. *)
+         (HSTEP1:Ir.SmallStep.sstep md1 st sr1)
+         (HSTEP2:Ir.SmallStep.sstep md2 st sr2),
+    Ir.Refinement.refines_step_res sr2 sr1. (* target refines source *)
+Proof.
+  intros.
+  inv HSTEP1.
+  { inv HSTEP2.
+    { inv HISTEP; try congruence.
+      unfold Ir.SmallStep.inst_det_step in HNEXT.
+      rewrite <- HINST1 in HNEXT.
+      rewrite HOP1 in HNEXT.
+      inv HISTEP0; try congruence.
+      unfold Ir.SmallStep.inst_det_step in HNEXT0.
+      rewrite <- HINST2 in HNEXT0.
+      rewrite HOP2 in HNEXT0.
+      inv HWF1.
+
+      (* okay.. time to do induction. *)
+      clear wf_cid_to_f.
+      clear wf_cid_to_f2.
+      clear wf_stack.
+      clear wf_no_bogus_ptr.
+      clear wf_no_bogus_ptr_mem.
+      induction HPP.
+      { (* base case *)
+        unfold Ir.deref in HNEXT.
+        destruct (Ir.get_deref m p1 (Ir.ty_bytesz retty)) eqn:HDEREF1.
+        { (* source is UB - it's done .*)
+          inv HNEXT. constructor. }
+        { inv HNEXT.
+          dup HDEREF1.
+          eapply Ir.get_deref_singleton in HDEREF0; try assumption.
+          {
+            destruct HDEREF0; try congruence.
+            destruct H. destruct H. inv H.
+            dup HDEREF1.
+            apply Ir.get_deref_ptr_phy_same with (p' := p2) in HDEREF1;
+              try assumption.
+            {
+              unfold Ir.deref in HNEXT0.
+              rewrite HDEREF1 in HNEXT0.
+              inv HNEXT0.
+              unfold Ir.load_val.
+              unfold Ir.load_bytes.
+              { rewrite HDEREF1. rewrite HDEREF0.
+                destruct x. destruct p.
+                constructor.
+                { constructor. }
+                { eapply eq_update_reg_and_incrpc2; try eassumption. }
+              }
+            }
+            { apply Ir.ty_bytesz_pos. }
+            { congruence. }
+          }
+          { apply Ir.ty_bytesz_pos. }
+        }
+      }
+      { (* a bit more complex case *)
+        admit.
+      }
+    }
+    { (* okay, br in target went wrong. *)
+      (* br in src shoud also go wrong. *)
+      apply Ir.Config.cur_inst_not_cur_terminator in HINST1.
+      inv HISTEP; try
+       (apply Ir.Config.cur_inst_not_cur_terminator in HINST2;
+        congruence).
+    }
+    { apply Ir.Config.cur_inst_not_cur_terminator in HINST2.
+      unfold Ir.SmallStep.t_step in HTSTEP.
+      rewrite <- HINST2 in HTSTEP.
+      congruence.
+    }
+  }
+  { apply Ir.Config.cur_inst_not_cur_terminator in HINST1.
+    unfold Ir.SmallStep.t_step in HTSTEP.
+    rewrite <- HINST1 in HTSTEP.
+    congruence. }
+  { apply Ir.Config.cur_inst_not_cur_terminator in HINST1.
+    unfold Ir.SmallStep.t_step in HTSTEP.
+    rewrite <- HINST1 in HTSTEP.
+    congruence. }
+Admitted.
+  
+
+End GVN.
+
+End Ir.
